\documentclass{article}

\usepackage{amsmath}

\title{Task 1. Lambda Term Reduction}
\author{Dmitriy Panfilyonok}
\date{}

\begin{document}
    \pagenumbering{gobble}
    \maketitle
    
    \paragraph{}
    \begin{align*}
        ((\lambda a.(\lambda b.bb)(\lambda b.bb))b)((\lambda c.(cb))(\lambda a.a))
        & = (\lambda a.(\lambda b.bb)(\lambda b.bb))b((\lambda c.cb)(\lambda a.a)) \\
        & \rightarrow_\beta (\lambda b.bb)(\lambda b.bb)((\lambda c.cb)(\lambda a.a)) \\
        & \rightarrow_\beta (\lambda b.bb)(\lambda b.bb)((\lambda a.a)b) \\
        & \rightarrow_\beta (\lambda b.bb)(\lambda b.bb)b \\
        & \rightarrow_\beta \ldots
    \end{align*}
    
\end{document}